Separate out path_embedding

src/graph_theory/minor.lean
@@ -4,169 +4,34 @@ open function
 open_locale classical
 
 namespace simple_graph
-    variables {V V' V'': Type}
-
-    structure path_embedding (G : simple_graph V) (G' : simple_graph V') :=
-        (f        : V ↪ V')
-        (df       : Π e : edges G, path G' (f e.x) (f e.y))
-        --
-        (nodup    : ∀ e : edges G, (df e).nodup)
-        (sym      : ∀ e : edges G, df e.flip = (df e).rev)
-        --
-        (endpoint : ∀ {e x},    f x ∈ df e              -> x ∈ e.ends)
-        (disjoint : ∀ {e e' z},   z ∈ df e -> z ∈ df e' -> e.ends = e'.ends ∨ ∃ x, z = f x)
-
-    def embeds_into (G : simple_graph V) (G' : simple_graph V') := nonempty (path_embedding G G')
-
-    namespace path_embedding
-        variables {G : simple_graph V} {G' : simple_graph V'} (F : path_embedding G G') {x y z : V}
-
-        lemma nop {e : edges G} : 0 < (F.df e).size
-            := by {
-                cases nat.eq_zero_or_pos (F.df e).size, swap, exact h, exfalso,
-                exact G.ne_of_adj e.h (F.f.injective (path.point_of_size_0 h))
-            }
-
-        def follow (p : path G x y) : path G' (F.f x) (F.f y)
-            := path.rec (λ _, path.point _) (λ _ _ _ h' _, path.concat (F.df ⟨h'⟩)) p
-
-        @[simp] lemma follow_point : follow F (path.point x) = path.point (F.f x) := rfl
-
-        @[simp] lemma follow_step {h : G.adj x y} {p : path G y z} : follow F (path.step h p) = path.concat (F.df ⟨h⟩) (follow F p) := rfl
-
-        lemma mem_follow {z} {p : path G x y} (h : 0 < p.size) : z ∈ follow F p <-> ∃ e ∈ p.edges, z ∈ F.df e
-            := by {
-                revert h, induction p with x' x' y' z' h' p' ih; simp, split; intro H,
-                    { cases H,
-                        { exact ⟨_, or.inl rfl, H⟩ },
-                        { cases p'; simp at *,
-                            { convert path.mem_tail },
-                            { cases (ih.mp H) with e he, exact ⟨e, or.inr he.1, he.2⟩ }
-                        }
-                    },
-                    { obtain ⟨e,H1,H2⟩ := H, cases H1,
-                        { left, subst H1, exact H2 },
-                        { right, cases p',
-                            { simp at H1, contradiction },
-                            { refine (ih _).mpr ⟨e,H1,H2⟩, simp }
-                        }
-                    }
-            }
-
-        lemma follow_nodup {p : path G x y} (h : p.nodup) : (follow F p).nodup
-            := by {
-                induction p with x' x' y' z' h' p' ih; simp [path.nodup_concat], rw path.nodup_step at h,
-                refine ⟨F.nodup _, ih h.2, _⟩, rintros u h3 h4,
-                cases nat.eq_zero_or_pos p'.size with h5 h5, { cases p', exact h4, simp at h5, contradiction },
-                obtain ⟨e,h7,h8⟩ := (mem_follow F h5).mp h4,
-                cases path.mem_edges h7, cases F.disjoint h3 h8 with h9 h9,
-                    { exfalso, apply h.1, apply (path.mem_of_edges h5).mpr ⟨e,h7,_⟩,
-                        rw <-h9, exact sym2.mem_mk_left _ _ },
-                    {
-                        obtain ⟨v,_⟩ := h9, subst u,
-                        have h10 := F.endpoint h3,
-                        cases sym2.mem_iff.mp h10 with h10 h10; simp at h10; subst h10,
-                        exfalso, apply h.1, cases sym2.mem_iff.mp (F.endpoint h8) with h12 h12;
-                        subst h12, exact left, exact right
-                    }
-            }
-
-        @[simp] lemma follow_append {p : path G x y} {h : G.adj y z} : follow F (p.append h) = (follow F p).concat (F.df ⟨h⟩)
-            := by { induction p; simp [*] }
-
-        lemma follow_rev {p : path G x y} : follow F p.rev = (follow F p).rev
-            := by {
-                induction p with x' x' y' z' h' p' ih, refl,
-                rw [follow_step,path.rev_step,follow_append,ih,path.concat_rev], congr,
-                set e : edges G := ⟨h'⟩, exact F.sym e
-            }
-    end path_embedding
-
-    namespace path_embedding
-        variables {G : simple_graph V} {G' : simple_graph V'} {G'' : simple_graph V''}
-
-        def comp (F : path_embedding G G') (F' : path_embedding G' G'') : path_embedding G G'' := {
-            f := ⟨F'.f ∘ F.f, injective.comp F'.f.inj' F.f.inj'⟩,
-            df := λ e, follow F' (F.df e),
-            --
-            nodup := λ e, (follow_nodup F') (F.nodup _),
-            sym := by { intro e, rewrite F.sym e, apply follow_rev },
-            --
-            endpoint := by {
-                intros e x h1, obtain ⟨e',h4,h5⟩ := (mem_follow F' (nop F)).mp h1,
-                exact F.endpoint ((path.mem_of_edges (nop _)).mpr ⟨e',h4,F'.endpoint h5⟩)
-            },
-            --
-            disjoint := by {
-                intros e e' z h1 h2,
-                replace h1 := (mem_follow _ (nop _)).mp h1, obtain ⟨e1,h3,h4⟩ := h1,
-                replace h2 := (mem_follow _ (nop _)).mp h2, obtain ⟨e2,h5,h6⟩ := h2,
-                have h7 := F'.disjoint h4 h6, cases h7,
-                {
-                    left, clear h4 h6,
-                    replace h3 := path.mem_edges h3,
-                    replace h5 := path.mem_edges h5,
-                    replace h5 : e1.x ∈ F.df e' ∧ e1.y ∈ F.df e' := by {
-                        cases edges.same_iff.mpr h7; subst e2,
-                        exact h5, simp at h5, exact h5.symm
-                    }, clear h7,
-                    cases F.disjoint h3.1 h5.1 with h10 h10, exact h10,
-                    obtain ⟨x,h10⟩ := h10, rw h10 at h3 h5,
-                    cases F.disjoint h3.2 h5.2 with h11 h11, exact h11,
-                    obtain ⟨y,h11⟩ := h11, rw h11 at h3 h5,
-                    have h12 := F.endpoint h3.1,
-                    have h13 := F.endpoint h3.2,
-                    have h14 := F.endpoint h5.1,
-                    have h15 := F.endpoint h5.2,
-                    have h16 : x ≠ y := by { intro h, apply G'.ne_of_adj e1.h, convert congr_arg F.f h },
-                    exact edges.sym2_eq h16 h12 h13 h14 h15
-                },
-                {
-                    obtain ⟨y,h8⟩ := h7, subst z,
-                    replace h4 := F'.endpoint h4,
-                    replace h6 := F'.endpoint h6,
-                    replace h3 := path.mem_edges h3,
-                    replace h5 := path.mem_edges h5,
-                    replace h3 : y ∈ F.df e, by { cases edges.mem_edge.mp h4; subst h, exact h3.1, exact h3.2 },
-                    replace h5 : y ∈ F.df e', by { cases edges.mem_edge.mp h6; subst h, exact h5.1, exact h5.2 },
-                    cases F.disjoint h3 h5 with h9 h9,
-                        { left, exact h9 },
-                        { obtain ⟨x,h9⟩ := h9, subst h9, right, use x, refl }
-                }
-            }
-        }
-
-        theorem trans : embeds_into G G' -> embeds_into G' G'' -> embeds_into G G''
-            := by { intros F F', cases F, cases F', use comp F F' }
-    end path_embedding
-
     namespace contraction
         structure setup :=
             {V : Type}
-            (G : simple_graph V)
-            (graph : simple_graph V)
-            (sub : ∀ {x y : V}, graph.adj x y -> G.adj x y)
+            (G g : simple_graph V)
+            (sub : ∀ {x y : V}, g.adj x y -> G.adj x y)
 
         variables (S : setup)
 
-        instance contraction_setoid : setoid S.V := ⟨S.graph.linked,simple_graph.linked.equiv⟩
+        instance contraction_setoid : setoid S.V := ⟨S.g.linked,simple_graph.linked.equiv⟩
 
         def clusters := quotient (contraction.contraction_setoid S)
+    end contraction
+
+    namespace contraction
+        variables {S : setup}
 
         def adj (x y : clusters S) := ∃ x' y' : S.V, x ≠ y ∧ ⟦x'⟧ = x ∧ ⟦y'⟧ = y ∧ S.G.adj x' y'
 
-        @[symm] lemma symm (x y : clusters S) : adj S x y -> adj S y x
+        @[symm] lemma symm (x y : clusters S) : adj x y -> adj y x
             := by { rintro ⟨x',y',h0,h1,h2,h3⟩, exact ⟨y',x',h0.symm,h2,h1,S.G.symm h3⟩ }
 
-        def contract : simple_graph (clusters S) := ⟨adj S, symm S⟩
+        def contract (S : setup) : simple_graph (clusters S) := ⟨adj, symm⟩
 
         lemma linked_of_adj {x y : S.V} (h : (contract S).adj ⟦x⟧ ⟦y⟧) : linked S.G x y
-            := by {
-                obtain ⟨a,b,h₁,h₂,h₃,h₄⟩ := h, transitivity b, transitivity a,
+            := by { obtain ⟨a,b,h₁,h₂,h₃,h₄⟩ := h, transitivity b, transitivity a,
                 exact linked_of_subgraph S.sub (quotient.eq.mp h₂.symm),
                 exact linked.edge h₄,
-                exact linked_of_subgraph S.sub (quotient.eq.mp h₃)
-            }
+                exact linked_of_subgraph S.sub (quotient.eq.mp h₃) }
 
         noncomputable def proj_path {x y : S.V} (p : path S.G x y) : path (contract S) ⟦x⟧ ⟦y⟧
             := path.rec (λ x, path.point ⟦x⟧) (λ x y z ha p ih, dite (⟦x⟧ = ⟦y⟧)
@@ -174,11 +39,8 @@ namespace simple_graph
                 (λ h, path.step ⟨x,y,h,rfl,rfl,ha⟩ ih)
             ) p
 
-        noncomputable def path_in_cluster {x y : S.V} (h : ⟦x⟧ = ⟦y⟧) : path S.graph x y
-            := path.to_path' (quotient.eq.mp h)
-
         lemma project_linked {S : setup} {x y : S.V} (h : linked S.G x y) : linked (contract S) ⟦x⟧ ⟦y⟧
-            := by { obtain ⟨p⟩ := path.to_path h, exact path.from_path ⟨proj_path S p⟩ }
+            := by { obtain ⟨p⟩ := path.to_path h, exact path.from_path ⟨proj_path p⟩ }
 
         lemma lift_linked' {S : setup} {xx yy : clusters S} (h : linked (contract S) xx yy) (x y : S.V)
                 (hx : ⟦x⟧ = xx) (hy : ⟦y⟧ = yy) : linked S.G x y
@@ -186,7 +48,7 @@ namespace simple_graph
                 induction h with x' xx' h1 h2 ih generalizing x y,
                 { subst hy, exact linked_of_subgraph S.sub (quotient.eq.mp hx) },
                 { obtain ⟨u, hu : ⟦u⟧ = x'⟩ := quot.exists_rep x', substs hu hx hy,
-                    transitivity u, exact ih x u rfl rfl, exact linked_of_adj S h2 }
+                    transitivity u, exact ih x u rfl rfl, exact linked_of_adj h2 }
             }
 
         lemma lift_linked {S : setup} {x y : S.V} (h : linked (contract S) ⟦x⟧ ⟦y⟧) : linked S.G x y
